coq/graph_model.v
@@ -2,6 +2,8 @@ Require Export lc.tactics.
 Require Import Coq.Logic.FunctionalExtensionality.
 Require Import lc.SetsAsPredicates.
 
+Require Import lc.env.
+
 (* https://github.com/jsiek/denotational_semantics/blob/master/agda/PValueCBV.agda *)
 
 
@@ -120,3 +122,337 @@ Qed.
 (* This is about primitive functions, so skip for now *)
 
 
+(* Environments ---------------------- *)
+
+Definition Env := GEnv (P Value).
+
+Definition ne (s : P Value) : Type := { x : Value & s x }.
+
+Definition nonempty_env (ρ : Env) : Type := forall x, ne (ρ x).
+
+(* Definition nonempty_env : Env -> Prop := fun ρ => forall x, Inhabited  _ (ρ x). *)
+
+Definition sub_env ( ρ1 : Env ) (ρ2: Env) : Prop :=
+  forall x, ρ1 x ⊆ ρ2 x.
+
+Infix "⊆e" := sub_env (at level 50).
+
+#[global] Instance Transitive_sub_env : Transitive sub_env.
+Proof. 
+  unfold Transitive. intros x y z S1 S2.
+  intros w. specialize (S1 w). specialize (S2 w).
+  transitivity (y w); auto.
+Qed.
+
+Import EnvNotations.
+
+Lemma extend_nonempty_env {ρ x X} : 
+  nonempty_env ρ -> ne X -> nonempty_env (x ⤇ X ● ρ).
+Proof.                                                
+  intros NEP NEX.
+  intro y. unfold env_cons.
+  destruct (x == y); eauto.
+Qed.
+
+Lemma env_ext {ρ ρ' y X} :
+  ρ ⊆e ρ' -> forall x , (y ⤇ X ● ρ) x ⊆ (y ⤇ X ● ρ' ) x.
+Proof. 
+  intros. unfold env_cons.
+  destruct (y == x); eauto. reflexivity.
+Qed.
+
+(* A finite environemtn has a list of values for 
+   each variable. *)
+Definition finite_env (ρ : Env) : Prop :=
+  forall x , exists E , (ρ x ≃ mem E) /\ E <> nil.
+
+Definition env_union (ρ1 ρ2 : Env) : Env := 
+  fun x v => ρ1 x v \/ ρ2 x v.
+
+Infix "⊔e" := env_union (at level 60).
+
+Lemma join_finite_env {ρ1 ρ2} : 
+  finite_env ρ1
+  -> finite_env ρ2
+  -> finite_env (ρ1 ⊔e ρ2).
+Proof. 
+  intros f1 f2 x.
+  move: (f1 x) => [E1 [ pE1 NE1 ]]. 
+  move: (f2 x) => [E2 [ pE2 NE2 ]].
+  exists (E1 ++ E2).
+  repeat split.
+  intros v [ p1x | p2x ].
+Admitted.
+
+Lemma join_lub {ρ ρ1 ρ2} :
+  ρ1 ⊆e ρ -> ρ2 ⊆e ρ -> (ρ1 ⊔e ρ2) ⊆e ρ.
+Proof.
+  intros p1p p2p x v [vp1x | vp2x].
+  eapply p1p; eauto.
+  eapply p2p; eauto.
+Qed.
+
+Lemma join_sub_left {ρ1 ρ2} : 
+  ρ1 ⊆e (ρ1 ⊔e ρ2).
+Proof.
+  intros x d z. left. eauto.
+Qed.
+
+Lemma join_sub_right {ρ1 ρ2} : 
+  ρ2 ⊆e (ρ1 ⊔e ρ2).
+Proof.
+  intros x d z. right. eauto.
+Qed.
+
+Definition monotone_env (D : Env -> P Value) := 
+ forall ρ ρ' , ρ ⊆e ρ' -> (D ρ) ⊆ D ρ'.
+
+(* --- Relations on results and products --------------- *)
+
+(* TODO.
+   This part seems to be not connected to the rest. 
+   Skipping for now.
+*)
+
+
+(* Continuous ----------------------------------------- *)
+
+Definition continuous_In (D:Env -> P Value) (ρ:Env) (v:Value) : Prop :=
+  v ∈ D ρ -> exists ρ' , finite_env ρ' /\ ρ' ⊆e ρ /\ (v ∈ D ρ').
+
+Definition continuous_env (D:Env -> P Value) (ρ:Env) : Prop :=
+  forall v, continuous_In D ρ v.
+
+(* creates an environment that maps each variable x to a singleton 
+   set of some element in ρ x *)
+Definition initial_finite_env (ρ : Env) (NE : nonempty_env ρ) : Env :=
+  fun x => match (NE x) with 
+        | existT _ y _ => ⌈ y ⌉
+        end.
+
+Lemma singleton_mem : forall v : Value,  ⌈ v ⌉ ⊆ mem (v :: nil).
+Proof. intro v. econstructor. inversion H. done. Qed.
+
+Lemma mem_singleton : forall v : Value, mem (v :: nil) ⊆ ⌈ v ⌉.
+Proof. intro v. cbv. intros. inversion H. subst. econstructor; eauto. done. Qed.
+
+#[global] Hint Resolve singleton_mem mem_singleton : core. 
+
+Lemma initial_fin (ρ : Env) (NE : nonempty_env ρ) :
+  finite_env (initial_finite_env ρ NE).
+Proof.
+  intros x.
+  unfold initial_finite_env.
+  unfold nonempty_env in NE.
+  move: (NE x) => [ v w ].
+  exists (cons v nil).
+  repeat split.
+  + eauto. 
+  + eauto.
+  + done.
+Qed.
+
+
+
+Lemma initial_fin_sub (ρ : Env) (NE : nonempty_env ρ) :
+  initial_finite_env ρ NE ⊆e ρ.
+Proof.
+  intros x y vinit.
+  unfold initial_finite_env in *.
+  unfold nonempty_env in NE.
+  destruct (NE x) as [v wpx].
+  inversion vinit. subst. auto.
+Qed.
+
+(* single-env maps x to D and any other variable y to something in ρ y. *)
+Definition single_env (x : atom) (D : P Value) (ρ : Env) (NE : nonempty_env ρ) : Env :=
+  fun y => match (x == y) with
+        | left _ => D
+        | right _ => let (v,_) := (NE y) in  ⌈ v ⌉
+        end.
+
+Lemma single_fin { v x ρ NE } : 
+  finite_env (single_env x ⌈ v ⌉ ρ NE).
+Proof.        
+  intros y. 
+  unfold single_env.
+  unfold nonempty_env in NE.
+  destruct (x == y).
+  + subst. exists (cons v nil).
+    repeat split; eauto. done.
+  + move: (NE y) => [ w _ ].
+    exists (cons w nil).
+    repeat split; eauto. done.
+Qed.
+
+Lemma single_sub { ρ x v } :
+  forall (NE : nonempty_env ρ),
+    v ∈ ρ x 
+  -> (single_env x ⌈ v ⌉ ρ NE) ⊆e ρ.
+Proof.
+  intros NE vpx y w sing.
+  unfold single_env in sing.
+  destruct (x == y).
+  + inversion sing. subst.
+    auto.
+  + destruct (NE y) as [u epy].
+    inversion sing. subst.
+    auto.
+Qed.
+
+(* v∈single[xv]x  *)
+Lemma v_single_xvx {v x ρ NE} : 
+  v ∈ single_env x ⌈ v ⌉ ρ NE x.
+Proof.
+  unfold single_env.
+  destruct (x == x). reflexivity. done.
+Qed.  
+
+Lemma mem_head a (V : list Value) :
+   a ∈ mem (a :: V).
+Proof. 
+  unfold mem. 
+  unfold Ensembles.In.
+  econstructor. auto.
+Qed.
+
+Lemma mem_cons d a (V : list Value) :
+    d ∈ mem V ->
+    d ∈ mem (a :: V).
+Proof. 
+  unfold mem. 
+  unfold Ensembles.In.
+  eapply in_cons.
+Qed.
+
+#[global] Hint Resolve mem_cons : core.
+
+(* continuous-∈⇒⊆ *)
+Lemma continuous_In_sub E ρ (NE : nonempty_env ρ) :
+   monotone_env E
+   -> forall V, mem V ⊆ E ρ
+   -> (forall v, v ∈ mem V -> continuous_In E ρ v)
+   -> exists ρ', finite_env ρ' /\ ρ' ⊆e ρ /\ (mem V ⊆ E ρ').
+Proof.
+  intros me V VE vcont.
+  induction V.
+  - exists (initial_finite_env ρ NE).
+    repeat split.
+    eapply (initial_fin ρ NE).
+    eapply initial_fin_sub; eauto. 
+    done.
+  - destruct IHV as [ ρ1 [ fρ1 [ ρ1ρ VEρ1 ]]].
+    intros d z. eapply VE; eauto.
+    intros v VM. eapply vcont; eauto.
+    destruct (vcont a) as [ρ2 [fρ2 [ρ2ρ VEρ2]]].
+    econstructor; eauto.
+    eapply VE. econstructor; eauto.
+    exists (ρ1 ⊔e ρ2).
+    repeat split.
+    eapply join_finite_env; eauto.
+    eapply join_lub; eauto.
+    intros d dm.
+    inversion dm; subst.
+    eapply me. eapply join_sub_right. eauto. 
+    eapply me. eapply join_sub_left. eauto.
+Qed.
+
+Lemma APPLY_continuous {D E ρ}{NE : nonempty_env ρ}{w} :
+    w ∈ ((D ρ) ▩ (E ρ))
+    -> continuous_env D ρ 
+    -> continuous_env E ρ
+    -> monotone_env D 
+    -> monotone_env E
+    -> exists ρ3 , 
+      finite_env ρ3 /\ ρ3 ⊆e  ρ 
+      /\ (w ∈ ((D ρ3) ▩ (E ρ3))).
+Proof.  
+  intros [V [VwDp [VEp VN]]].
+  intros IHD IHE mD mE.
+  destruct (IHD (V ↦ w) VwDp) as 
+    [ ρ1 [ fρ1 [ ρ1ρ VwDp1 ]]].
+  destruct 
+    (continuous_In_sub E ρ NE mE V VEp)
+      as [ ρ2 [ fρ2 [ ρ2ρ VEp2 ]]].
+  intros v vV. eapply IHE; eauto.
+  exists (ρ1 ⊔e ρ2).
+  repeat split.
+  - eapply join_finite_env; eauto.
+  - eapply join_lub; eauto.
+  - exists V. 
+    have VwDp3 : V ↦ w ∈ D (ρ1 ⊔e ρ2).
+    { eapply mD. 2: eapply VwDp1. 
+      intros x v z. left.  auto. }
+    have VEρ3 : mem V ⊆ E (ρ1 ⊔e ρ2).
+    { intros v vV. eapply mE.
+      2: eapply VEp2; auto. 
+      intros x m z. right. auto. }
+    repeat split.
+    + auto.
+    + auto.
+    + done.
+Qed.
+
+
+Lemma env_tail {ρ' x v ρ} :  
+  ρ' ⊆e (x ⤇ v ● ρ) -> finite_env ρ' -> 
+  nonempty_env ρ ->
+  exists w, exists ρ'', ρ' = (x ⤇ w ● ρ'') /\
+                (w ⊆ v) /\
+                ρ'' ⊆e ρ /\
+                finite_env ρ''.
+Proof.
+  intros h k ne.
+  move: (ne x) => [ vv I ].
+  exists (ρ' x). exists (x ⤇ ⌈ vv ⌉ ● ρ'). 
+  repeat split.
+  + extensionality y.
+    unfold env_cons. destruct (x == y). subst. auto. auto.
+  + move: (h x) => ll. unfold env_cons in ll. 
+    rewrite eq_dec_refl in ll. auto.
+  + intros y. move: (h y) => ll.
+    unfold env_cons in *.
+    destruct (x == y). subst.  
+    cbv. intros x hh. inversion hh. subst. auto. auto.
+  + unfold finite_env in *.
+    intros y.
+      unfold env_cons.
+      destruct (x == y). subst.
+      exists (cons vv nil). split. cbv.
+      split. intros x h0. inversion h0. auto.
+      intros x h0. destruct h0. subst. reflexivity. done.
+      done.
+      destruct (k y) as [E [F G]].
+      exists E. split; auto.
+Qed.
+
+Lemma Lambda_continuous {E ρ} {NE : nonempty_env ρ}{ v x} :
+  v ∈ Λ (fun D => E (x ⤇ D ● ρ)) 
+  -> (forall V, V <> nil -> 
+          continuous_env E (x ⤇ mem V ● ρ))
+  -> monotone_env E
+  -> exists ρ', finite_env ρ' /\
+            ρ' ⊆e ρ /\
+            (v ∈ (Λ (fun D => E (x ⤇ D ● ρ')))).
+Proof.
+  induction v.
+  - intro h. inversion h.
+  - intros [ wEVρ VN ] IH mE.
+    destruct (IH l VN v wEVρ) as
+      [ ρ' [ fρ' [ ρ'Vρ wEρ' ]]]. 
+    edestruct (env_tail ρ'Vρ fρ' NE) as 
+      [ w [ ρ'' [ EQ [ WV [ S T]]]]].
+    exists ρ''. subst.
+    repeat split.
+    + auto.
+    + auto.
+    + eapply mE; eauto. 
+      intros y.
+      unfold env_cons.
+      destruct (x == y); auto. reflexivity.
+    + done.
+  - exists (initial_finite_env ρ NE).
+    repeat split.
+    eapply (initial_fin ρ NE).
+    eapply (initial_fin_sub ρ NE).
+Qed.
