coq/env.v
@@ -1,0 +1,41 @@
+Require Export lc.tactics.
+Require Export lc.relations.
+Require Import Coq.Logic.FunctionalExtensionality.
+
+Import LCNotations.
+Local Open Scope lc_scope.
+
+Section Env.
+
+Variable Value : Type.
+
+Polymorphic Definition GEnv := atom -> Value.
+
+Definition env_cons : atom -> Value -> GEnv -> GEnv := 
+  fun x v γ => fun y => match (x == y) with 
+                  | left _ => v
+                  | right pf => γ y
+                  end.
+
+Lemma cons_cons : forall x y z v γ, 
+    z <> y ->
+    z <> x ->
+    env_cons y ((env_cons z v γ) x) (env_cons z v γ) = env_cons z v (env_cons y (γ x) γ).
+Proof.
+  intros.
+  unfold env_cons.
+  extensionality w.
+  destruct (y == w) eqn:YW;
+  destruct (z == w) eqn:ZW; auto.
+  + subst. done. 
+  + subst. destruct (z == x). subst. done. done.
+Qed.     
+
+End Env.
+
+Arguments env_cons {_}.
+Arguments cons_cons {_}.
+
+Module EnvNotations.
+Notation "x ⤇ v ● ρ" := (env_cons x v ρ) (at level 60).
+End EnvNotations.
